HoareLogic/ProgramState.v
@@ -1,5 +1,4 @@
 Require Import Coq.Relations.Relation_Operators.
-Require Import Logic.lib.SigStream.
 Require Import Logic.PropositionalLogic.KripkeSemantics.
 Require Import Logic.SeparationLogic.SeparationAlgebra.
 
@@ -144,5 +143,4 @@ Proof.
   intros.
   destruct mb, ma; auto; simpl in *; congruence.
 Qed.
-
 
