lib/Stream/SigStream.v
@@ -47,95 +47,6 @@ Tactic Notation "stream_extensionality" ident(x) :=
      apply stream_extensionality; intro x
   end.
 
-Definition partial_stream_len {A: Type} (h: stream A) (n: nat): option nat :=
-  match h n with
-  | Some _ => None
-  | None => Some
-    ((fix f (m: nat): nat :=
-       match h m with
-       | Some _ => S m
-       | None => match m with
-                 | 0 => 0
-                 | S m0 => f m0
-                 end
-       end) n)
-  end.
-
-Lemma partial_stream_len_mono1: forall {A: Type} (h: stream A) (x y: nat), x <= y -> partial_stream_len h y = None -> partial_stream_len h x = None.
-Proof.
-  intros.
-  unfold partial_stream_len in *.
-  destruct (h y) eqn:?H; try congruence.
-  pose proof (stream_sound2 h x y H) as [? ?]; [eauto |].
-  rewrite H2; auto.
-Qed.
-
-Lemma partial_stream_len_mono2: forall {A: Type} (h: stream A) (x y n: nat), x <= y -> partial_stream_len h x = Some n -> partial_stream_len h y = Some n.
-Proof.
-  intros.
-  unfold partial_stream_len in *.
-  destruct (h x) eqn:?H; try congruence.
-  pose proof (stream_sound1 h x y H H1).
-  inversion H0.
-  rewrite H2, H4; clear H0.
-  f_equal.
-  revert n H4; induction H; intros; auto.
-  pose proof (stream_sound1 h x m H H1).
-  specialize (IHle H0 _ H4).
-  rewrite IHle; clear IHle.
-  rewrite H2; auto.
-Qed.
-
-Program Definition stream_app {A: Type} (h1 h2: stream A): stream A :=
-  fun n: nat =>
-    match partial_stream_len h1 n return option A with
-    | None => h1 n
-    | Some m => h2 (n - m)
-    end.
-Next Obligation.
-  destruct (partial_stream_len h1 x) eqn:?H.
-  + pose proof H1.
-    apply (partial_stream_len_mono2 h1 x y n) in H1; [| omega].
-    rewrite H1.
-    apply (stream_sound1 h2 (x - n) (y - n)); auto.
-    omega.
-  + unfold partial_stream_len in H1.
-    rewrite H0 in H1.
-    congruence.
-Qed.
-
-Fixpoint partial_stream_clen {A: Type} (h: nat -> stream A) (n: nat): nat * nat :=
-  match n with
-  | 0 => (0, 0)
-  | S n => let (k, m) := partial_stream_clen h n in
-           match h k (S m) with
-           | Some _ => (k, S m)
-           | None => (S k, 0)
-           end
-  end.
-
-Fixpoint partial_stream_clen' {A: Type} (h: nat -> stream A) (n: nat): option (nat * nat) :=
-  let (k, m) := partial_stream_clen h n in
-  match n with
-  | 0 => match h k m with
-         | Some _ => Some (k, m)
-         | None => None
-         end
-  | S n => match h k m, partial_stream_clen' h n with
-           | Some _, Some _ => Some (k, m)
-           | _, _ => None
-           end
-  end.
-
-Program Definition stream_capp {A: Type} (h: nat -> stream A): stream A :=
-  fun n: nat =>
-    match partial_stream_clen' h n return option A with
-    | Some (k, m) => h k m
-    | None => None
-    end.
-Next Obligation.
-Admitted.
-
 Definition is_fin_stream {A: Type} (h: stream A): Prop :=
   exists n, h n = None.
 
@@ -148,20 +59,10 @@ Definition is_n_stream {A: Type} (n: nat) (h: stream A): Prop :=
 Definition is_at_least_n_stream {A: Type} (n: nat) (h: stream A): Prop :=
   forall n', n' < n -> h n' <> None.
 
+Definition is_empty_stream {A: Type}: stream A -> Prop :=
+  is_n_stream 0.
+
 (*
-Definition fin_stream {A: Type} (h: list A) : stream A.
-  exists (fun n => nth_error h n).
-  intros.
-  rewrite nth_error_None_iff in H0 |- *.
-  omega.
-Defined.
-
-Definition inf_stream {A: Type} (h: nat -> A) : stream A.
-  exists (fun n => Some (h n)).
-  intros.
-  congruence.
-Defined.
-
 Definition fstn_stream {A: Type} (n: nat) (h: stream A) : stream A.
   exists (fun m => if le_lt_dec n m then None else h m).
   intros.
